README.md
@@ -7,6 +7,7 @@ Features:
 - **Compiler checked PromQL:** PromQL queries are checked during compilation. Many aspects of a dashboard panel can be automatically set based on the query.
 - **Models for exporters and targets:** A model (e.g. for node-exporter) contains all metrics, incl. types, units, help strings, and possible label names. Queries can be checked against this model.
 - The units of panels can be automatically set based on the query. E.g. if a metric is in bytes and you wrap it into `rate()` the unit of the panel will be bytes/second.
+- Easily create a topk queries over time laveraging Grafana variables.
 - **Extensible:** awesome-dashboards is written in Lean 4. Also dashboards are written directly in Lean. You have the full power of a dependently-typed language at your fingertips.
 - **Opt out:** If you no longer want to use this library, you can simply maintain your dashboard in Grafana.
 - **Dashboard preview in the IDE:** Lean 4 supports widgets in the IDE. This can be used to preview the dashboard.
