hack/run-grafana.sh
@@ -6,7 +6,7 @@ SCRIPT_DIR=$( cd -- "$( dirname -- "${BASH_SOURCE[0]}" )" &> /dev/null && pwd )
 
 docker rm -f grafana
 docker run -d \
-    -v $SCRIPT_DIR/grafana/datasources.yaml:/etc/grafana/provisioning/datasources/datasources.yaml \
-    -v $SCRIPT_DIR/grafana/source1.yaml:/etc/grafana/provisioning/dashboards/source1.yaml \
-    -v $SCRIPT_DIR/grafana/dashboards/:/dashboards \
+    -v $SCRIPT_DIR/../grafana/datasources.yaml:/etc/grafana/provisioning/datasources/datasources.yaml \
+    -v $SCRIPT_DIR/../grafana/source1.yaml:/etc/grafana/provisioning/dashboards/source1.yaml \
+    -v $SCRIPT_DIR/../grafana/dashboards/:/dashboards \
     --name grafana --net host grafana/grafana
